proofs/isabelle/SpecRest/Codegen.thy
@@ -49,6 +49,7 @@ export_code
     peel_smt_relation_ref
     peel_relation_ref_full
     type_expr_to_ty
+    type_expr_full_to_ty
     schema_field_type
     schema_relation_value_type
     tyctx_empty
